src/QueryStructure/Refinements/ConstraintChecksRefinements.v
@@ -1,36 +1,570 @@
-Require Export QueryStructureNotations QueryQSSpecs ListImplementation.
-Require Import List Compare_dec AdditionalLemmas AdditionalPermutationLemmas AdditionalMorphisms EnsembleListEquivalenceProperties flattenCompListProperties.
+Require Export QueryStructureNotations QueryQSSpecs.
+Require Import List Compare_dec AdditionalLemmas
+        AdditionalPermutationLemmas AdditionalMorphisms
+        EnsembleListEquivalenceProperties flattenCompListProperties
+        GeneralQueryRefinements.
 
 Unset Implicit Arguments.
 
 Transparent Count Query_For.
 
+Section ConstraintCheckRefinements.
+  Hint Resolve AC_eq_nth_In AC_eq_nth_NIn crossConstr.
+  Hint Unfold SatisfiesCrossRelationConstraints
+       SatisfiesSchemaConstraints.
+
+  Fixpoint app_assoc {A : Set} (As As' As'' : list A):
+      As ++ (As' ++ As'') = (As ++ As') ++ As'' :=
+    match As as As return
+                  As ++ (As' ++ As'') = (As ++ As') ++ As'' with
+              | [] => eq_refl _
+              | a :: As => (f_equal (fun l => a :: l) (app_assoc As As' As''))
+            end.
+
+  Lemma app_comm_cons' {A : Set}:
+    forall (a : A) As As',
+      As ++ (a :: As') = (As ++ [a]) ++ As'.
+  Proof.
+    intros; rewrite <- app_assoc; reflexivity.
+  Defined.
+
+  Definition Ensemble_BoundedIndex_app_comm_cons {A : Set}
+    (a : A)
+    (As As' : list A)
+    (P : Ensemble (BoundedIndex (As ++ a :: As')))
+  : Ensemble (BoundedIndex ((As ++ [a]) ++ As')).
+    rewrite app_comm_cons' in P; exact P.
+  Defined.
+
+  Definition BoundedIndex_app_comm_cons {A : Set}
+    (a : A)
+    (As As' : list A)
+    (a' : BoundedIndex (As ++ a :: As'))
+  : BoundedIndex ((As ++ [a]) ++ As').
+    rewrite app_comm_cons' in a'; exact a'.
+  Defined.
+
+  Lemma ibound_BoundedIndex_app_comm_cons {A : Set}
+    (a : A)
+    (As As' : list A)
+    (a' : BoundedIndex (As ++ a :: As'))
+  : ibound a' = ibound (BoundedIndex_app_comm_cons a As As' a').
+  Proof.
+    unfold BoundedIndex_app_comm_cons, eq_rec, eq_rect; simpl.
+    destruct (app_comm_cons' a As As'); reflexivity.
+  Qed.
+
+  Program Fixpoint Iterate_Ensemble_BoundedIndex'
+          {A : Set}
+          (Visited Remaining : list A)
+          (P : Ensemble (BoundedIndex (Visited ++ Remaining))) : Prop :=
+    match Remaining with
+        | [] => True
+        | a :: Remaining' =>
+          P {| bindex := a;
+               indexb := {| ibound := List.length Visited;
+                            boundi := _ |} |}
+          /\ Iterate_Ensemble_BoundedIndex' (Visited ++ (a :: nil)) Remaining' _
+    end.
+  Next Obligation.
+    clear P; induction Visited; simpl; auto.
+  Defined.
+  Next Obligation.
+    exact (Ensemble_BoundedIndex_app_comm_cons _ _ _ P).
+  Defined.
+
+  Lemma Ensemble_BoundedIndex_app_equiv {A : Set}
+        (A_eq_dec : forall a a' : A, {a = a'} + {a <> a'})
+        (a : A) (As As' : list A)
+        (P : Ensemble (BoundedIndex (As ++ a :: As')))
+  : forall idx idx' n nth nth',
+      P {| bindex := idx; indexb := {| ibound := n; boundi := nth |}|} <->
+      Ensemble_BoundedIndex_app_comm_cons a As As' P
+                                     {| bindex := idx'; indexb := {| ibound := n; boundi := nth' |}|}.
+  Proof.
+    split; unfold Ensemble_BoundedIndex_app_comm_cons, BoundedIndex_app_comm_cons, app_comm_cons'; simpl;
+    unfold eq_rec, eq_rect, eq_ind, eq_rect; destruct (app_assoc As [a] As'); auto;
+    generalize (indexb_ibound_eq
+            {| bindex := idx'; indexb := {| ibound := n; boundi := nth' |}|}
+            {| bindex := idx; indexb := {| ibound := n; boundi := nth |}|}
+            eq_refl); simpl; intros; subst;
+    erewrite (eq_proofs_unicity_Opt_A A_eq_dec _); eauto.
+  Qed.
+
+  Lemma BoundedIndex_app_comm_cons_nth_eq {A : Set}
+        (A_eq_dec : forall a a' : A, {a = a'} + {a <> a'})
+  : forall
+      (As As' : list A)
+      a a' a'' n nth nth',
+      {| bindex := a; indexb := {| ibound := n; boundi := nth |}|} =
+      BoundedIndex_app_comm_cons a' As As' {| bindex := a''; indexb := {| ibound := n; boundi := nth' |}|}.
+  Proof.
+    intros.
+    unfold BoundedIndex_app_comm_cons, eq_rec, eq_rect; simpl.
+    destruct (app_comm_cons' a' As As').
+    generalize (indexb_ibound_eq
+            {| bindex := a''; indexb := {| ibound := n; boundi := nth' |}|}
+            {| bindex := a; indexb := {| ibound := n; boundi := nth |}|}
+               eq_refl); simpl; intros; subst.
+    erewrite (eq_proofs_unicity_Opt_A A_eq_dec nth'); reflexivity.
+  Qed.
+
+  Lemma Ensemble_BoundedIndex_nth_eq {A : Set}
+        (A_eq_dec : forall a a' : A, {a = a'} + {a <> a'})
+  : forall
+      (As : list A)
+      (P : Ensemble (BoundedIndex As))
+      a a' n nth nth',
+      P {| bindex := a; indexb := {| ibound := n; boundi := nth |}|} ->
+      P {| bindex := a'; indexb := {| ibound := n; boundi := nth' |}|}.
+  Proof.
+    intros;
+    generalize (indexb_ibound_eq
+            {| bindex := a'; indexb := {| ibound := n; boundi := nth' |}|}
+            {| bindex := a; indexb := {| ibound := n; boundi := nth |}|}
+               eq_refl); simpl; intros; subst.
+    erewrite (eq_proofs_unicity_Opt_A A_eq_dec nth'); eassumption.
+  Qed.
+
+  Lemma nth_error_app {A : Set} :
+    forall (a : A) (As As' : list A) n,
+      nth_error As n = Some a ->
+      nth_error (As ++ As') n = Some a.
+  Proof.
+    induction As; destruct n; simpl; intros; try discriminate; auto.
+  Defined.
+
+  Lemma Ensemble_nth_error_app
+        {A : Set}
+        (A_eq_dec : forall a a' : A, {a = a'} + {a <> a'})
+  : forall a (As As' : list A) nth'
+      (P : Ensemble (BoundedIndex (As ++ (a :: As')))),
+      P {| bindex := a;
+           indexb := {| ibound := Datatypes.length As;
+                        boundi := nth' |} |}
+      -> (forall (a' : A) (n : nat) (nth : nth_error As n = Some a'),
+      P {| bindex := a';
+           indexb := {|
+                      ibound := n;
+                      boundi := nth_error_app _ As (a :: As') n nth |} |})
+      -> forall (a' : A) (n : nat) (nth : nth_error (As ++ [a]) n = Some a'),
+           Ensemble_BoundedIndex_app_comm_cons a As As' P
+                                          {| bindex := a';
+                                             indexb := {| ibound := n;
+                                                          boundi := nth_error_app _ (As ++ [a]) As' n nth |} |}.
+  Proof.
+    intros.
+    destruct (eq_nat_dec (List.length As) n ); subst.
+    - rewrite (BoundedIndex_app_comm_cons_nth_eq
+                 A_eq_dec As As' _ _ _  (List.length As)
+                 (nth_error_app _ (As ++ [a]) As'
+                                (Datatypes.length As) nth)
+                 nth').
+      erewrite <- BoundedIndex_app_comm_cons_nth_eq; eauto.
+      eapply Ensemble_BoundedIndex_app_equiv; eauto.
+    - assert (nth_error As n = Some a') by
+          (revert n nth n0; clear; induction As; destruct n; simpl; intros;
+           try congruence;
+           [destruct n; discriminate
+           | eauto]).
+      generalize (H0 _ _ H1); intros.
+      erewrite (BoundedIndex_app_comm_cons_nth_eq
+                 A_eq_dec As As' _ _ _ n
+                 (nth_error_app _ (As ++ [a]) As'
+                                n nth)).
+      erewrite <- BoundedIndex_app_comm_cons_nth_eq; eauto.
+      eapply Ensemble_BoundedIndex_app_equiv; eauto.
+      Grab Existential Variables.
+      rewrite <- app_assoc; simpl; apply nth_error_app; eassumption.
+      apply nth_error_app; eassumption.
+      apply nth_error_app; eassumption.
+  Qed.
+
+  Lemma Iterate_Ensemble_equiv' {A : Set}
+        (A_eq_dec : forall a a' : A, {a = a'} + {a <> a'})
+  : forall (Remaining Visited : list A)
+           (P : Ensemble (BoundedIndex (Visited ++ Remaining))),
+      (forall a n (nth : nth_error Visited n = Some a),
+         P {| bindex := a;
+              indexb := {| ibound := n;
+                           boundi := nth_error_app _ _ _ _ nth |} |})
+      -> (Iterate_Ensemble_BoundedIndex' Visited Remaining P ->
+         forall idx, P idx).
+    intros; destruct idx as [idx [n nth_n] ]; simpl in *.
+    revert Visited P H H0 idx n nth_n; induction Remaining; simpl; intros.
+    - eapply Ensemble_BoundedIndex_nth_eq with (a := idx); auto.
+    - split_and.
+      assert (nth_error ((Visited ++ [a]) ++ Remaining) n = Some idx)
+        as nth_n'
+          by (rewrite <- app_assoc; simpl; assumption).
+      generalize (IHRemaining _ _ (Ensemble_nth_error_app A_eq_dec _ _ _ _ P H1 H) H2 _ _ nth_n').
+      unfold Ensemble_BoundedIndex_app_comm_cons, eq_rect; destruct (app_comm_cons' a Visited Remaining).
+      intros; erewrite (eq_proofs_unicity_Opt_A A_eq_dec nth_n); eauto.
+      Grab Existential Variables.
+      rewrite app_nil_r in nth_n; assumption.
+  Qed.
+
+  Lemma Iterate_Ensemble_equiv'' {A : Set}
+        (A_eq_dec : forall a a' : A, {a = a'} + {a <> a'})
+  : forall (Remaining Visited : list A)
+           (P : Ensemble (BoundedIndex (Visited ++ Remaining))),
+      (forall idx, P idx)
+      -> Iterate_Ensemble_BoundedIndex' Visited Remaining P.
+    induction Remaining; simpl; auto.
+    intros; split; eauto.
+    eapply IHRemaining; intros; eauto.
+    intros; destruct idx as [idx [n nth_n] ]; simpl in *.
+    eapply Ensemble_BoundedIndex_app_equiv; eauto.
+    Grab Existential Variables.
+    rewrite <- app_assoc in nth_n; simpl in nth_n; eassumption.
+  Qed.
+
+  Definition Iterate_Ensemble_BoundedIndex
+          (Bound : list string)
+          (P : Ensemble (BoundedIndex Bound)) : Prop :=
+    Iterate_Ensemble_BoundedIndex' [] Bound P.
+
+
+  Program Lemma refine_Iterate_Ensemble {A : Set}
+        (A_eq_dec : forall a a' : A, {a = a'} + {a <> a'})
+  : forall (As : list string)
+           (P : Ensemble (BoundedIndex As)),
+      refine {b | decides b (forall idx : BoundedIndex As, P idx)}
+             {b | decides b (@Iterate_Ensemble_BoundedIndex As P)}.
+  Proof.
+    intros; eapply refine_pick_pick.
+    intros; destruct x; simpl in *.
+    intros; eapply Iterate_Ensemble_equiv' with (Visited := []);
+    eauto using string_dec.
+    destruct n; simpl; intros; discriminate.
+    unfold not; intros; apply H.
+    apply Iterate_Ensemble_equiv'';
+      auto using string_dec.
+  Qed.
+
+  (* So that things play nicely with setoid rewriting *)
+  Definition If_Then_Else {A}  (b : bool) (t e : A)
+    := if b then t else e.
+
+  Program Fixpoint Iterate_Decide_Comp' (A : Set)
+          (Remaining Visited : list A)
+          (P : Ensemble (BoundedIndex (Visited ++ Remaining)))
+          {struct Remaining }
+  : Comp bool :=
+    match Remaining with
+      | nil => ret true
+      | cons a Remaining' =>
+        Bind {b' |
+              decides b' (P {| bindex := a;
+                               indexb := {| ibound := List.length Visited;
+                                            boundi := _ |} |})}%comp
+             (fun b' =>
+                If_Then_Else b'
+                             (Iterate_Decide_Comp' _ Remaining' (Visited ++ [a]) _)
+                             (ret false))
+    end.
+  Next Obligation.
+    clear P; induction Visited; simpl; auto.
+  Defined.
+  Next Obligation.
+    exact (Ensemble_BoundedIndex_app_comm_cons _ _ _ P).
+  Defined.
+
+  Lemma refine_Iterate_Decided_Ensemble' {A : Set}
+        (A_eq_dec : forall a a' : A, {a = a'} + {a <> a'})
+  : forall (Remaining Visited : list A)
+           (P : Ensemble (BoundedIndex (Visited ++ Remaining))),
+      refine {b | decides b (Iterate_Ensemble_BoundedIndex' Visited Remaining P)}
+             (Iterate_Decide_Comp' _ Remaining Visited P).
+  Proof.
+    induction Remaining; simpl; intros.
+    - econstructor; inversion_by computes_to_inv; subst; simpl; auto.
+    - econstructor; apply computes_to_inv in H; destruct_ex;
+      split_and; inversion_by computes_to_inv; subst.
+      destruct x; simpl in *.
+      {  destruct v; simpl in *; intuition; intros; eauto.
+         - generalize (IHRemaining (Visited ++ [a]) _ _ H1).
+           intros; inversion_by computes_to_inv; simpl in *; eauto.
+         - generalize (IHRemaining (Visited ++ [a]) _ _ H1).
+           intros; inversion_by computes_to_inv; simpl in *; eauto.
+      }
+      { inversion_by computes_to_inv; subst; simpl; intuition. }
+  Qed.
+
+  Lemma decides_True :
+    refine {b | decides b True}%comp
+           (ret true).
+  Proof.
+    econstructor; inversion_by computes_to_inv; subst; simpl; auto.
+  Qed.
+
+  Lemma decides_2_True (A : Type) (B : A -> Type) :
+    refine {b' | decides b' (forall a : A, B a -> True)}%comp
+           (ret true).
+  Proof.
+    econstructor; inversion_by computes_to_inv; subst; simpl; auto.
+  Qed.
+
+  Lemma decides_3_True (A B : Type) (C : B -> Type) :
+    refine {b' | decides b' (A -> forall b : B, C b -> True)}%comp
+           (ret true).
+  Proof.
+    econstructor; inversion_by computes_to_inv; subst; simpl; auto.
+  Qed.
+
+  Lemma decides_neq (A : Type) (B : Prop) (a : A) :
+    refine {b' | decides b' (a <> a -> B)}%comp
+           (ret true).
+  Proof.
+    econstructor; inversion_by computes_to_inv; subst; simpl; auto.
+    congruence.
+  Qed.
+
+  Global Add Parametric Morphism A
+  : If_Then_Else
+      with signature
+      (@eq bool) ==> (@refine A) ==> (@refine A) ==> (@refine A)
+        as refine_If_Then_Else_if.
+  Proof.
+    compute.
+    intros; destruct_head bool; intros; eauto.
+  Qed.
+
+  Definition Iterate_Decide_Comp
+          (Bound : list string)
+          (P : Ensemble (BoundedIndex Bound))
+  : Comp bool :=
+    Iterate_Decide_Comp' _ Bound [] P.
+
+  Definition Iterate_Decide_Comp_BoundedIndex
+  : forall (Bound : list string)
+           (P : Ensemble (BoundedIndex Bound)),
+      refine {b | decides b (forall Ridx', P Ridx')}
+             (Iterate_Decide_Comp _ P).
+  Proof.
+    intros.
+    setoid_rewrite refine_Iterate_Ensemble; auto using string_dec.
+    setoid_rewrite refine_Iterate_Decided_Ensemble'; auto using string_dec.
+    reflexivity.
+  Qed.
+
+  (* Consequences of ith_replace_BoundIndex_neq and ith_replace_BoundIndex_eq on updates *)
+
+  Lemma refine_SatisfiesSchemaConstraints_self
+  : forall qsSchema
+           (Ridx : @BoundedString (map relName (qschemaSchemas qsSchema)))
+           (tup tup' : @Tuple (schemaHeading (QSGetNRelSchema qsSchema Ridx))),
+      refine {b | decides b (SatisfiesSchemaConstraints Ridx tup tup')}
+             match (schemaConstraints (QSGetNRelSchema qsSchema Ridx)) with
+                 Some Constr => {b | decides b (Constr tup tup') }
+               | None => ret true
+             end.
+  Proof.
+    unfold SatisfiesSchemaConstraints.
+    intros; destruct (schemaConstraints (QSGetNRelSchema qsSchema Ridx));
+    eauto using decides_True.
+    reflexivity.
+  Qed.
+
+  Lemma refine_SatisfiesSchemaConstraints
+  : forall qsSchema qs
+           (Ridx : @BoundedString (map relName (qschemaSchemas qsSchema)))
+           (tup : @Tuple (schemaHeading (QSGetNRelSchema qsSchema Ridx))),
+      refine {b | decides b
+                          (forall tup',
+                             GetUnConstrRelation qs Ridx tup'
+                             -> SatisfiesSchemaConstraints Ridx tup tup')}
+             match (schemaConstraints (QSGetNRelSchema qsSchema Ridx)) with
+                 Some Constr =>
+                 {b | decides b (forall tup',
+                                   GetUnConstrRelation qs Ridx tup'
+                                   -> Constr tup tup')}
+               | None => ret true
+             end.
+  Proof.
+    unfold SatisfiesSchemaConstraints.
+    intros; destruct (schemaConstraints (QSGetNRelSchema qsSchema Ridx));
+    eauto using decides_True.
+    reflexivity.
+    apply decides_2_True.
+  Qed.
+
+  Lemma refine_SatisfiesSchemaConstraints'
+  : forall qsSchema qs
+           (Ridx : @BoundedString (map relName (qschemaSchemas qsSchema)))
+           (tup : @Tuple (schemaHeading (QSGetNRelSchema qsSchema Ridx))),
+      refine {b | decides b
+                          (forall tup',
+                             GetUnConstrRelation qs Ridx tup'
+                             -> SatisfiesSchemaConstraints Ridx tup' tup)}
+             match (schemaConstraints (QSGetNRelSchema qsSchema Ridx)) with
+                 Some Constr =>
+                 {b | decides b (forall tup',
+                                   GetUnConstrRelation qs Ridx tup'
+                                   -> Constr tup' tup)}
+               | None => ret true
+             end.
+  Proof.
+    unfold SatisfiesSchemaConstraints.
+    intros; destruct (schemaConstraints (QSGetNRelSchema qsSchema Ridx));
+    eauto using decides_True.
+    reflexivity.
+    apply decides_2_True.
+  Qed.
+
+  Definition Ensemble_opt_BoundedIndex_app_comm_cons {A : Set}
+    (a : A)
+    (As As' : list A)
+    (P : BoundedIndex (As ++ a :: As') -> option Prop)
+  : BoundedIndex ((As ++ [a]) ++ As') -> option Prop.
+    rewrite app_comm_cons' in P; exact P.
+  Defined.
+
+  Program Fixpoint Iterate_Decide_Comp_opt' (A : Set)
+          (Remaining Visited : list A)
+          (P : BoundedIndex (Visited ++ Remaining) -> option Prop )
+          {struct Remaining }
+  : Comp bool :=
+    match Remaining with
+      | nil => ret true
+      | cons a Remaining' =>
+        match (P {| bindex := a;
+                    indexb := {| ibound := List.length Visited;
+                                 boundi := _ |} |}) with
+          | Some P' => b' <- {b' | decides b' P'};
+                      If_Then_Else b'
+                                   (Iterate_Decide_Comp_opt' _ Remaining' (Visited ++ [a])
+                                                             (Ensemble_opt_BoundedIndex_app_comm_cons _ _ _ P))
+                                   (ret false)
+          | None => (Iterate_Decide_Comp_opt' _ Remaining' (Visited ++ [a])
+                                              (Ensemble_opt_BoundedIndex_app_comm_cons _ _ _ P))
+        end
+    end%comp.
+  Next Obligation.
+    clear P; induction Visited; simpl; auto.
+  Defined.
+
+  Lemma refine_Iterate_Decide_Comp'
+        {A : Set}
+        (A_eq_dec : forall a a' : A, {a = a'} + {a <> a'})
+  : forall (Remaining Visited : list A)
+           (P : BoundedIndex (Visited ++ Remaining)
+                -> option Prop),
+      refine (@Iterate_Decide_Comp' _ Remaining Visited (fun idx => match P idx with
+                                                                      | Some P' => P'
+                                                                      | None => True
+                                                                    end))
+             (@Iterate_Decide_Comp_opt' _ Remaining Visited P).
+    induction Remaining; simpl; intros.
+    - reflexivity.
+    - destruct (P ``(a)).
+      + f_equiv; unfold pointwise_relation; intros.
+        destruct a0; simpl; try reflexivity.
+        setoid_rewrite <- IHRemaining; f_equiv.
+        unfold Ensemble_BoundedIndex_app_comm_cons,
+        Ensemble_opt_BoundedIndex_app_comm_cons; simpl.
+        destruct (app_comm_cons' a Visited Remaining); simpl.
+        reflexivity.
+      + rewrite decides_True; simplify with monad laws; simpl.
+        setoid_rewrite <- IHRemaining; f_equiv.
+        unfold Ensemble_BoundedIndex_app_comm_cons,
+        Ensemble_opt_BoundedIndex_app_comm_cons; simpl.
+        destruct (app_comm_cons' a Visited Remaining); simpl.
+        reflexivity.
+  Qed.
+
+  Lemma refine_Iterate_Decide_Comp
+  : forall (Bound : list string)
+           (P : BoundedIndex Bound -> option Prop),
+      refine (@Iterate_Decide_Comp _ (fun idx => match P idx with
+                                                 | Some P' => P'
+                                                 | None => True
+                                               end))
+             (@Iterate_Decide_Comp_opt' _ Bound [] P).
+  Proof.
+    intros; unfold Iterate_Decide_Comp;
+    rewrite refine_Iterate_Decide_Comp'.
+    reflexivity.
+    apply string_dec.
+  Qed.
+
+  Lemma refine_SatisfiesCrossConstraints
+  : forall qsSchema qs
+           (Ridx : @BoundedString (map relName (qschemaSchemas qsSchema)))
+           (tup : @Tuple (schemaHeading (QSGetNRelSchema qsSchema Ridx))),
+      refine
+        (@Iterate_Decide_Comp _
+                              (fun Ridx' =>
+                                 SatisfiesCrossRelationConstraints
+                                   Ridx Ridx' tup
+                                   (GetUnConstrRelation qs Ridx')))
+        (@Iterate_Decide_Comp_opt' _ _ []
+                                   (fun Ridx' =>
+                                      match (BuildQueryStructureConstraints qsSchema Ridx Ridx') with
+                                        | Some CrossConstr =>
+                                          Some (CrossConstr tup (GetUnConstrRelation qs Ridx'))
+                                        | None => None
+                                      end)) .
+  Proof.
+    intros.
+    setoid_rewrite <- refine_Iterate_Decide_Comp.
+    unfold SatisfiesCrossRelationConstraints; f_equiv.
+    apply functional_extensionality; intros.
+    destruct BuildQueryStructureConstraints; reflexivity.
+  Qed.
+
+  Lemma refine_Iterate_Decide_Comp_equiv
+        {A : Set}
+        (A_eq_dec : forall a a' : A, {a = a'} + {a <> a'})
+  : forall (Remaining Visited : list A)
+           (P P' : Ensemble (BoundedIndex (Visited ++ Remaining))),
+      (forall idx, P idx -> P' idx) ->
+      (forall idx, ~ P idx -> ~ P' idx) ->
+      refine (@Iterate_Decide_Comp' _ Remaining Visited P')
+             (@Iterate_Decide_Comp' _ Remaining Visited P).
+  Proof.
+    induction Remaining; simpl; intros.
+    - reflexivity.
+    - f_equiv.
+      + unfold refine; intros; inversion_by computes_to_inv; subst;
+        econstructor; destruct v; simpl in *; eauto.
+      + unfold pointwise_relation; intros b; destruct b; simpl.
+        apply IHRemaining.
+        unfold Ensemble_BoundedIndex_app_comm_cons; simpl;
+        destruct (app_comm_cons' a Visited Remaining); simpl; eauto.
+        unfold Ensemble_BoundedIndex_app_comm_cons; simpl;
+        destruct (app_comm_cons' a Visited Remaining); simpl; eauto.
+        reflexivity.
+  Qed.
+
+End ConstraintCheckRefinements.
+
 Lemma For_computes_to_In :
   forall {heading} P,
     (forall a, P a \/ ~ P a) ->
     forall seq ens,
-      computes_to (For (QueryResultComp (heading := heading) ens 
+      computes_to (For (QueryResultComp (heading := heading) ens
                                         (fun tup => Where (P tup) Return tup))) seq ->
-      forall x, 
+      forall x,
         List.In x seq -> (P x /\ (exists x0, ens x0 /\ indexedTuple x0 = x)).
 Proof.
-  unfold refine, decides, Count, Query_In, UnConstrQuery_In,  Query_Where, Query_Return; 
+  unfold refine, decides;
   unfold Query_For, QueryResultComp; intros * excl;
   induction seq as [ | head seq' IH ]; intros.
-  
+
   exfalso; intuition.
-  
+
   inversion_by computes_to_inv.
-  
+
   pose proof (permutation_cons_in H4) as in_x0.
   apply in_split in in_x0.
-  destruct in_x0 as [ x0_before [ x0_after ? ] ]; subst. 
+  destruct in_x0 as [ x0_before [ x0_after ? ] ]; subst.
   symmetry in H4. apply Permutation_cons_app_inv in H4.
 
   rewrite map_map in H5.
   destruct (flatten_CompList_app_cons_inv _ excl _ _ _ _ H5) as [ x1_before [ x1_middle [ head' [ x1_after (_eq & in_orig & before & middle & after) ] ] ] ]; subst.
-  
-  unfold boxed_option in middle; simpl in middle. 
+
+  unfold boxed_option in middle; simpl in middle.
   apply computes_to_inv in middle.
   destruct middle as [head'' (middle1 & middle2)].
   apply computes_to_inv in middle1.
@@ -52,31 +586,31 @@ Proof.
 
   - subst x; split; [ | exists head'; split; [ apply H3  | ] ]; auto.
   - pose proof (EnsembleListEquivalence_slice _ _ _ H3) as smaller_equiv.
-    pose proof (flatten_CompList_app _ _ _ _ before after) as flatten_app. 
+    pose proof (flatten_CompList_app _ _ _ _ before after) as flatten_app.
     set (smaller_ens := (fun x : IndexedTuple => ens x /\ ~ In x x1_middle)).
     split.
 
     + eapply H1; try assumption.
-      econstructor; [ | constructor; symmetry; eassumption ]. 
+      econstructor; [ | constructor; symmetry; eassumption ].
       econstructor.
-      constructor. 
+      constructor.
 
       apply smaller_equiv.
 
       unfold boxed_option in *.
       rewrite !map_app, !map_map.
-      apply flatten_app. 
+      apply flatten_app.
     + assert (exists x0 : IndexedTuple, smaller_ens x0 /\ indexedTuple x0 = x) as temp.
       apply H2; try eassumption.
-      econstructor; [ | constructor; symmetry; eassumption ]. 
+      econstructor; [ | constructor; symmetry; eassumption ].
       econstructor.
-      constructor. 
+      constructor.
 
       eassumption.
       unfold boxed_option in *.
       rewrite !map_app, !map_map.
-      apply flatten_app. 
-      
+      apply flatten_app.
+
       destruct temp as [ x0 ( ens_x & _eq ) ]; subst.
       eexists; split; eauto.
 
@@ -87,20 +621,19 @@ Qed.
 Lemma For_computes_to_nil :
   forall {heading} P,
   forall ens,
-    computes_to (For (QueryResultComp (heading := heading) ens 
+    computes_to (For (QueryResultComp (heading := heading) ens
                                       (fun tup => Where (P tup) Return tup))) [] ->
     forall x,
       ens x -> ~ (P (indexedTuple x)).
 Proof.
-  unfold refine, decides, Count, Query_In, UnConstrQuery_In,  Query_Where, Query_Return; 
-  unfold Query_For, QueryResultComp; intros **.
+  unfold refine, decides, Count, Query_For, QueryResultComp; intros **.
 
                                             inversion_by computes_to_inv.
   symmetry in H2; apply Permutation_nil in H2; subst.
   apply H1 in H0.
   apply in_split in H0.
   destruct H0 as [ x1_before [ x1_after _eq ] ]; subst.
-  
+
   rewrite map_map in H3.
   eapply flatten_CompList_nil; unfold boxed_option; eauto; intuition.
 Qed.
@@ -122,7 +655,7 @@ Lemma refine_constraint_check_into_query :
                decides b
                        (exists tup2: @IndexedTuple _,
                           (GetUnConstrRelation c tbl tup2 /\ P (indexedTuple tup2)))))
-      (Bind 
+      (Bind
          (Count (For (UnConstrQuery_In c tbl (fun tup => Where (P tup) Return tup))))
          (fun count => ret (negb (beq_nat count 0)))).
 Proof.
@@ -134,7 +667,7 @@ Proof.
   destruct (Datatypes.length x0) eqn:eq_length;
     destruct x0 as [ | head tail ]; simpl in *; try discriminate; simpl.
 
-  pose proof (For_computes_to_nil _ (GetUnConstrRelation c tbl) H0). 
+  pose proof (For_computes_to_nil _ (GetUnConstrRelation c tbl) H0).
   rewrite not_exists_forall; intro a; rewrite not_and_implication; intros.
   apply H; trivial.
 
@@ -145,7 +678,7 @@ Proof.
   apply decidable_excl; assumption.
 Qed.
 
-Definition refine_foreign_key_check_into_query {schm tbl} := 
+Definition refine_foreign_key_check_into_query {schm tbl} :=
   @refine_constraint_check_into_query schm tbl.
 
 Require Import tupleAgree Bool AdditionalRefinementLemmas.
@@ -160,7 +693,7 @@ Lemma refine_functional_dependency_check_into_query :
        (forall tup' : IndexedTuple,
           ~ (GetUnConstrRelation c tbl tup' /\ tupleAgree ref tup' args1 /\ ~ tupleAgree ref tup' args2))) ->
       refine
-        (Pick (fun (b : bool) => 
+        (Pick (fun (b : bool) =>
                  decides b
                          (forall tup' : IndexedTuple,
                             GetUnConstrRelation c tbl tup' ->
@@ -178,14 +711,14 @@ Proof.
 
   setoid_replace (forall tup', GetUnConstrRelation c tbl tup' ->
                                tupleAgree ref tup' args1 -> tupleAgree ref tup' args2)
-  with           (forall tup', ~ (GetUnConstrRelation c tbl tup' /\ 
-                                  tupleAgree ref tup' args1 /\ 
+  with           (forall tup', ~ (GetUnConstrRelation c tbl tup' /\
+                                  tupleAgree ref tup' args1 /\
                                   ~ tupleAgree ref tup' args2)); eauto.
 
   setoid_rewrite refine_decide_negation.
   setoid_rewrite tupleAgree_equivalence.
   setoid_rewrite (refine_constraint_check_into_query
-                    (fun (x: Tuple ) => tupleAgree_computational ref x args1 /\ 
+                    (fun (x: Tuple ) => tupleAgree_computational ref x args1 /\
                                         ~ tupleAgree_computational ref x args2)); try assumption.
 
   Opaque Query_For Count.
@@ -193,3 +726,54 @@ Proof.
   setoid_rewrite negb_involutive.
   reflexivity.
 Qed.
+
+Lemma tupleAgree_refl :
+  forall (h : Heading)
+         (tup : @Tuple h)
+         (attrlist : list (Attributes h)),
+    tupleAgree tup tup attrlist.
+Proof.
+  unfold tupleAgree; auto.
+Qed.
+
+Lemma refine_tupleAgree_refl_True :
+  forall (h : Heading)
+         (tup : @Tuple h)
+         (attrlist attrlist' : list (Attributes h)),
+    refine {b |
+            decides b (tupleAgree tup tup attrlist'
+                       -> tupleAgree tup tup attrlist)}
+           (ret true).
+Proof.
+  unfold refine; intros; inversion_by computes_to_inv.
+  subst; econstructor; simpl; auto using tupleAgree_refl.
+Qed.
+
+Ltac simplify_trivial_SatisfiesSchemaConstraints :=
+  simpl;
+  try rewrite refine_tupleAgree_refl_True;
+  try setoid_rewrite decides_True;
+  try setoid_rewrite decides_2_True; reflexivity.
+
+Ltac simplify_trivial_SatisfiesCrossRelationConstraints :=
+  simpl map; simpl;
+    repeat match goal with
+             | |- context [if _ then ret true else ret false] =>
+               setoid_rewrite refine_if_bool_eta at 1
+             | |- refine (Bind (Pick (fun b => decides b True)) _) _ =>
+             etransitivity; [ apply refine_bind;
+                              [ apply decides_True
+                              | unfold pointwise_relation;
+                                intro; higher_order_1_reflexivity ]
+                            | rewrite refineEquiv_bind_unit at 1;
+                              unfold If_Then_Else ]
+             | |- refine (Bind (Pick (fun b' => decides b' (forall _ _ _, True))) _ ) _ =>
+               etransitivity;
+                 [ apply refine_bind;
+                   [ apply decides_3_True
+                   | unfold pointwise_relation;
+                     intro; higher_order_1_reflexivity ]
+                 | rewrite refineEquiv_bind_unit at 1;
+                   unfold If_Then_Else ]
+
+    end.
