src/QueryStructure/Refinements/OperationRefinements.v
@@ -1,0 +1,3 @@
+Require Export GeneralInsertRefinements GeneralQueryRefinements
+        GeneralQueryStructureRefinements ConstraintChecksRefinements
+        ConstraintChecksUnfoldings.
